Updates

high2/Zeta.High.Interleave.fst
@@ -156,7 +156,7 @@ let eac_value_is_evicted_value (#app #n:_) (il: eac_log app n) (gk: key app):
                   eac_state_evicted_value es = eac_value gk il))
   = admit()
 
-let ext_evict_val_is_stored_val (#app #n:_) (il: eac_log app n) (i: seq_index il):
+let ext_evict_val_is_stored_val (#app #n:_) (il: verifiable_log app n) (i: seq_index il):
   Lemma (requires (V.is_evict (I.index il i)))
         (ensures (let tid = I.src il i in
                   let st_pre = thread_store_pre tid il i in
