high2/Zeta.High.Interleave.fsti
@@ -196,7 +196,7 @@ let value_ext (#app:_) (ee: vlog_entry_ext app {EvictMerkle? ee \/ EvictBlum? ee
     | EvictMerkle _ v -> v
     | EvictBlum _ v _ -> v
 
-val ext_evict_val_is_stored_val (#app #n:_) (il: eac_log app n) (i: seq_index il):
+val ext_evict_val_is_stored_val (#app #n:_) (il: verifiable_log app n) (i: seq_index il):
   Lemma (requires (V.is_evict (I.index il i)))
         (ensures (let tid = I.src il i in
                   let st_pre = thread_store_pre tid il i in
